src/Ast/Resolver.dfy
@@ -4,18 +4,35 @@ module Resolver {
     provides Wrappers, Raw, Ast
 
   import opened Std.Wrappers
-  import Types
+  import opened Basics
+  import opened Types
   import Raw = RawAst
-  import Ast
+  import opened Ast
 
   method Resolve(b3: Raw.Program) returns (r: Result<Ast.Program, string>)
     ensures r.Success? ==> b3.WellFormed()
   {
-    var types := {};
-    for i := 0 to |b3.types| {
-      var typename := b3.types[i];
-      var typ := new Types.Type(typename);
-      types := types + {typ};
+    var boolType := new Type(BoolTypeName);
+    var intType := new Type(IntTypeName);
+    var typeMap := map[BoolTypeName := boolType, IntTypeName := intType];
+    for n := 0 to |b3.types|
+      invariant BuiltInTypes <= typeMap.Keys
+      invariant forall i :: 0 <= i < n ==> b3.types[i] in typeMap.Keys && b3.types[i] !in BuiltInTypes
+      invariant MapIsInjective(typeMap)
+      invariant forall i, j :: 0 <= i < j < n ==> b3.types[i] != b3.types[j]
+    {
+      var typename := b3.types[n];
+      if typename in typeMap.Keys {
+        return Failure("duplicate type name: " + typename);
+      }
+      var typ := new Type(typename);
+      typeMap := typeMap[typename := typ];
+    }
+    assert forall typ <- b3.types :: typ !in BuiltInTypes;
+    assert forall i, j :: 0 <= i < j < |b3.types| ==> b3.types[i] != b3.types[j];
+
+    if |b3.procedures| == 0 { // TODO
+      return Success(Program(typeMap.Values, {}));
     }
 
     return Failure("good so far, but resolver is not yet fully implemented");
